cartogtrapjhy verifies under 4.11.1+13bdccd7cab58c0dd087e82dde654db04fab657 (= lately) but not postconditions

TRUMP.dfy
@@ -2,6 +2,251 @@
 include "Ownership-Parallel.dfy"
 
 
+lemma SETIN(left : Owner, right : Owner)
+  requires forall f <- left :: f in right
+   ensures left <= right
+{}
+
+lemma SETLREQ(left : Owner, right : Owner)
+  requires left <= right
+  requires left >= right
+   ensures left == right
+{}
+
+//{:timeLimit 30} {:timeLimit 60}
+lemma cartography(owner : Owner, pivot : Object)
+//topology?  enfringement?  whatevs?
+  returns (owners_inside : Owner, owners_outside : Owner, flat_below : Owner, fringe : Owner)
+
+ requires AllReady(flatten(owner))
+ requires pivot.Ready()     requires piR: pivot.Ready()
+
+  ensures owners_inside  == set x <- owner |  inside(x, pivot)
+  ensures owners_outside == set x <- owner | outside(x, pivot)
+  ensures owner == owners_outside + owners_inside
+  ensures flatten(owner) == flatten(owners_inside) + flatten(owners_outside)
+
+  ensures flat_below == set x <- flatten(owners_inside) | inside(x,pivot)
+  ensures fringe     == set x <- flatten(owners_inside), xo <- x.owner | (x != pivot) &&  (inside(x,pivot) ) && (outside(xo,pivot) ) :: xo
+
+  ensures reveal froglet(); froglet(owner, pivot, owners_inside, owners_outside, flat_below, fringe)
+  ensures flatten(owner) == flatten(owners_outside) + flat_below + flatten(fringe) + pflivot(owner, pivot)
+
+  ensures owners_inside <= flat_below
+  ensures flat_below <= flatten(owners_inside)
+
+{
+  makerfield(owner,pivot);
+  owners_inside  := set x <- owner |  inside(x, pivot);
+  owners_outside := set x <- owner | outside(x, pivot);
+  assert FLOOI: flatten(owner) == flatten(owners_outside) + flatten(owners_inside);
+
+// //////////////////////////////////////////////////////////////////////////////////////////////////////////
+//   assert flatten(owner) == flatten(owners_outside) + flatten(owners_inside);
+//   assert flatten(owners_outside) == flatten(set x <- owner | outside(x, pivot));
+//   assert flatten(owners_inside) == flat_inside_nopivot + pflivot(owner, pivot);
+//   assert flat_inside_nopivot == flat_below + flat_above;
+//   assert flatten(owners_inside) ==
+//   assert flat_above == flatten(whole_f) == flatten(fringe) + flatten(pivot_f)
+//   assert flat_below ==
+//
+//   assert flatten(owner) == flatten(owners_outside) + flat_below + flatten(fringe) + pflivot(owner, pivot);
+//   assert reveal froglet(); froglet(owner, pivot, owners_inside, owners_outside, flat_below, fringe);
+//   return;
+//////////////////////////////////////////////////////////////////////////////////////////////////////////
+
+
+
+  if (owners_inside == {})
+  {
+    flat_below := {}; fringe := {};
+    assert owners_outside == owner;
+
+    assert flatten(owner) == flatten(owners_outside) + flat_below + flatten(fringe) + pflivot(owner, pivot);
+    assert reveal froglet(); froglet(owner, pivot, owners_inside, owners_outside, flat_below, fringe);
+    return;
+  }
+
+
+  if (owners_inside == {pivot})
+  {
+    flat_below := {pivot}; fringe := {};
+    assert owners_outside == owner - {pivot};
+
+    assert flat_below == {pivot};
+    assert flatten(fringe) == {};
+    assert flatten(owner) == flatten(owners_outside) + {pivot} + {} + pflivot(owner, pivot);
+
+    assert flatten(owner) == flatten(owners_outside) + flat_below + flatten(fringe) + pflivot(owner, pivot);
+    assert reveal froglet(); froglet(owner, pivot, owners_inside, owners_outside, flat_below, fringe);
+    return;
+  }
+
+//the pivot MAY be within owners_inside - but only if it's in the actual "owner" argument
+//otherwise the pivot won't be in owners_inside
+//BUT: the pivot (and its flattening) most certainly will be in flatten(owners_inside)
+//because every one or the owners_inside is inside the pivot (by definiton)
+
+
+
+  assert flatten(owners_outside) == flatten(set x <- owner | outside(x, pivot));
+
+  assert owners_inside > {};
+
+  assert exists o <- owners_inside :: strictlyInside(o,pivot);
+
+  var owners_inside_nopivot := owners_inside - {pivot};
+  assert owners_inside_nopivot > {};  //implied by strictlyInside above
+
+  if (pivot in owner) {
+    assert pivot in owners_inside;
+    assert owners_inside_nopivot + {pivot} == owners_inside;
+    FLATTEN_SUM3(owners_inside_nopivot, {pivot}, owners_inside);
+    assert flatten(owners_inside_nopivot) + flatten({pivot}) == flatten(owners_inside);
+    assert pflivot(owner, pivot) == flatten({pivot});
+    assert flatten(owners_inside_nopivot) + pflivot(owner, pivot) == flatten(owners_inside);
+  }
+  else
+  {
+    assert pivot !in owners_inside;
+    assert owners_inside_nopivot == owners_inside;
+    assert flatten(owners_inside_nopivot) + {} == flatten(owners_inside);
+    assert pflivot(owner, pivot) == {};
+    assert flatten(owners_inside_nopivot) + pflivot(owner, pivot) == flatten(owners_inside);
+  }
+
+    assert flatten(owners_inside) == flatten(owners_inside_nopivot) + pflivot(owner, pivot);
+
+
+  var flat_inside_nopivot := flatten(owners_inside_nopivot);
+   assert pivot in flat_inside_nopivot;
+   FlattenContainsFlatten(owners_inside_nopivot,{pivot});
+   assert flatten({pivot}) <= flat_inside_nopivot;    ///yes but htis pivot stems from one of the owners_inside_nopivot --- not pivot itself listed seperately
+    assert flatten(owners_inside) == flat_inside_nopivot + pflivot(owner, pivot);
+
+
+      flat_below := set x <- flat_inside_nopivot | inside(x,pivot);   ///pivot will be inside
+  var flat_above := set x <- flat_inside_nopivot | outside(x,pivot);  //do I need this one?
+  makerfield(flat_inside_nopivot,pivot);
+  assert flat_inside_nopivot == flat_below + flat_above;
+
+
+var whole_f;
+var pivot_f;
+
+//do I ned this call here - or can I just convert the following asserts into assignments?
+whole_f,fringe,pivot_f := GordonRamseyThemFringes(owners_inside_nopivot, pivot);
+// perhaops better to turn this around, have the definitions here,
+//   and the pass them into as lemma, rather than getting them out of the lemma?
+
+
+//jun05 2026
+// assert   whole_f  == set x  <- flat_inside_nopivot, xo <- x.owner |                  (inside(x,pivot) ) && (outside(xo,pivot) ) :: xo;
+// assert   fringe   == set x  <- flat_inside_nopivot, xo <- x.owner | (x != pivot) &&  (inside(x,pivot) ) && (outside(xo,pivot) ) :: xo;
+// assert   pivot_f  == set x  <- flat_inside_nopivot, xo <- x.owner | (x == pivot) &&  (inside(x,pivot) ) && (outside(xo,pivot) ) :: xo;
+ assert  forall x <- flat_inside_nopivot |  inside(x,pivot)  :: x in flat_below;
+assert  forall x <- flat_below :: (x in  flat_inside_nopivot) && inside(x,pivot);
+
+// assert (set x <- flat_below) == (set x <- flat_inside_nopivot |  inside(x,pivot));
+//
+// assert   whole_f  == set x : Object <- flat_below, xo <- x.owner  |                                     && (outside(xo,pivot) ) :: xo;
+// assert   fringe   == set x : Object <- flat_below, xo <- x.owner  | (x != pivot)                        && (outside(xo,pivot) ) :: xo;
+// assert   pivot_f  == set x : Object <- flat_below, xo <- x.owner  | (x == pivot)                        && (outside(xo,pivot) ) :: xo;
+
+assert pivot_f + fringe == whole_f;
+FLATTEN_SUM3(pivot_f,fringe,whole_f);
+assert flatten(pivot_f) + flatten(fringe) == flatten(whole_f);
+assert pivot_f == pivot.owner;   assert PIVOT_FO: pivot_f == pivot.owner;
+
+
+// assert flatten(whole_f)  == flat_above;
+
+assert forall w <- whole_f :: outside(w,pivot);
+
+  forall t <- flat_above ensures (t in (flatten(fringe) + flatten(pivot_f)))   // (t in flatten(fringe)) //(t in flatten(fringe))  //by
+  {
+    forall part <- owners_inside_nopivot | (t in flatten({part})) ensures (t in (flatten(fringe) + flatten(pivot_f))) {
+      var prev, next := AcrossTheBorder(part, pivot, t);
+      assert strictlyInside(prev,t);
+      assert not(strictlyInside(next,pivot)); //ORIG
+      assert prev in flatten(owners_inside_nopivot);
+      assert next in prev.owner;
+      assert prev in flat_below;
+      assert (next in flat_above) || (next == pivot);
+      assert (next in fringe) || (next == pivot);
+      assert t in flatten(owners_inside_nopivot);
+      assert t in next.AMFO;
+      assert t in flatten({next});
+      if (next in fringe) { assert t in flatten(fringe); }
+       else { assert next == pivot; assert t in flatten(pivot_f); }
+      assert t in (flatten(fringe) + flatten(pivot_f));
+    }
+  }
+
+  assert forall t <- flat_above ::(t in (flatten(fringe) + flatten(pivot_f)));
+
+  assert ((flatten(fringe) + flatten(pivot_f)) >= flat_above);
+
+  assert FPGE: ((flatten(fringe) + flatten(pivot.owner)) >= flat_above) by { reveal PIVOT_FO; }
+
+  assert forall f <- flatten(fringe) :: f in flat_above;
+  assert forall f <- flatten(pivot.owner) :: f in flat_above;
+  assert forall f <- (flatten(fringe) + flatten(pivot.owner)) :: f in flat_above;
+  SETIN((flatten(fringe) + flatten(pivot.owner)), flat_above);
+  assert FPLE: (flatten(fringe) + flatten(pivot.owner)) <= flat_above;
+
+  assert flat_above == (flatten(fringe) + flatten(pivot.owner)) by
+   {
+    reveal FPGE;  assert (flatten(fringe) + flatten(pivot.owner )) >= flat_above;
+    reveal FPLE;  assert (flatten(fringe) + flatten(pivot.owner)) <= flat_above;
+    SETLREQ((flatten(fringe) + flatten(pivot.owner)), flat_above);
+   }
+  assert      flat_above == (flatten(fringe) + flatten(pivot.owner));
+  assert FAB: flat_above == (flatten(fringe) + flatten(pivot.owner));
+
+  assert flat_inside_nopivot == flat_below + flat_above;
+  assert flat_inside_nopivot == flat_below +  (flatten(fringe) + flatten(pivot.owner))
+       by { reveal FAB;
+            assert flat_above ==( (flatten(fringe) + flatten(pivot.owner)));
+            assert flat_inside_nopivot == flat_below +  (flatten(fringe) + flatten(pivot.owner)); }
+
+
+ assert flatten(owners_outside) == flatten(set x <- owner | outside(x, pivot));
+
+ assert flatten(owners_inside) == flatten(owners_inside_nopivot) + pflivot(owner, pivot);
+ assert flatten(owners_inside) == flat_inside_nopivot + pflivot(owner, pivot);
+ assert flatten(owners_inside) == (flat_below + flat_above) + pflivot(owner, pivot);
+ assert flatten(owners_inside) == (flat_below +   (flatten(fringe) + flatten(pivot.owner))  ) + pflivot(owner, pivot);
+
+ assert BFPL: flatten(owners_inside) == (flat_below +   (flatten(fringe) + flatten(pivot.owner))  ) + pflivot(owner, pivot);
+
+//  assert flatten(owners_inside) == ((set x <- flat_inside_nopivot | inside(x,pivot))  + (flatten(fringe) + flatten(pivot.owner))  ) + pflivot(owner, pivot);
+
+
+
+  assert flatten(owner) == flatten(owners_outside) + flatten(owners_inside) by { reveal FLOOI; }
+  assert flatten(owner) == flatten(owners_outside) + flat_below + flatten(fringe) + flatten(pivot.owner) + pflivot(owner, pivot)
+    by {
+         reveal FLOOI;
+         assert flatten(owner) == flatten(owners_outside) + flatten(owners_inside);
+         reveal BFPL;
+         assert flatten(owners_inside) ==                  (flat_below + (flatten(fringe) + flatten(pivot.owner))) + pflivot(owner, pivot);
+         SATAN(owner, owners_outside, owners_inside, flat_below, fringe, pivot);
+         assert flatten(owner) == flatten(owners_outside) + flat_below +  flatten(fringe) + flatten(pivot.owner)   + pflivot(owner, pivot);
+        }
+
+//  assert flatten(owner) == flatten(owners_outside) + (flat_below + (flatten(fringe) + flatten(pivot.owner))) + pflivot(owner, pivot);
+//  assert flatten(owner) == flatten(owners_outside) +  flat_below +  flatten(fringe) + flatten(pivot.owner)   + pflivot(owner, pivot);
+//   // assert froglet(owner, pivot, owners_inside, owners_outside, flat_below, fringe) by { reveal froglet(); }
+  // assert froglet(owner, pivot, owners_inside, owners_outside, flat_below, fringe);
+  }
+
+lemma SATAN(owner : Owner, owners_outside : Owner, owners_inside : Owner, flat_below : Owner, fringe : Owner, pivot : Object)
+ requires flatten(owner) == flatten(owners_outside) + flatten(owners_inside)
+ requires flatten(owners_inside) == (flat_below + (flatten(fringe) + flatten(pivot.owner))) + pflivot(owner, pivot);
+  ensures flatten(owner) == flatten(owners_outside) + flat_below +  flatten(fringe) + flatten(pivot.owner)   + pflivot(owner, pivot);
+{}
+
 
 lemma fromTheManyOne(less : seq<nat>, more : seq<nat>)
   requires |less| == |more|
@@ -11,6 +256,22 @@ lemma fromTheManyOne(less : seq<nat>, more : seq<nat>)
 
 function sum(s : seq<int>) : int
 { if (|s| == 0) then 0 else s[0] + sum(s[1..]) }
+
+
+lemma FLATTEN_OWNER(o : Object)
+  requires o.Ready()
+   ensures flatten(o.owner) == o.AMFX
+   ensures flatten({o}) == o.AMFO  >= flatten(o.owner)
+{}
+
+
+lemma FLATTEN_OWNER2(o : Object, oo : Object)
+  requires o.Ready()
+  requires oo.Ready()
+  requires oo in o.owner
+   ensures flatten(o.owner) == o.AMFX
+   ensures flatten({o}) == o.AMFO  >= flatten(o.owner) >= flatten({oo})
+{}
 
 
 
@@ -168,7 +429,7 @@ lemma farage(ownrs : OWNR, aliens : Owner)
 
 
 lemma farage3(ownrs : OWNR, othrs : OWNR, aliens : Owner)
- //given aliaes in flattern(ownrs), faltten(alianes) in flattern(owners)
+ //given aliaes in flattern(ownrs), faltten(alianes) in flattern(owners
   requires AllReady((ownrs))
   requires AllReady((othrs))
   requires AllReady((aliens))
@@ -197,7 +458,7 @@ lemma farage3(ownrs : OWNR, othrs : OWNR, aliens : Owner)
 
 
 lemma {:timeLimit 30} makerfield(ownrs : OWNR, pivot : Object)
-  requires AllReady(flatten(ownrs))
+  requires AllReady(ownrs)   //was   requires AllReady(flatten(ownrs))
   requires pivot.Ready()
    ensures forall x <- ownrs ::    (x.AMFO >= pivot.AMFO) != (not(x.AMFO >= pivot.AMFO))
    ensures forall x <- ownrs :: not(x.AMFO >= pivot.AMFO) != not(not(x.AMFO >= pivot.AMFO))
@@ -205,7 +466,18 @@ lemma {:timeLimit 30} makerfield(ownrs : OWNR, pivot : Object)
    ensures forall x <- ownrs ::           inside(x,pivot) != not( inside(x,pivot))
    ensures forall x <- ownrs ::
         not(strictlyInside(x,pivot)) == (outside(x,pivot) || (x == pivot))
+   ensures ownrs == (set x <- ownrs | inside(x,pivot)) + (set x <- ownrs | outside(x,pivot))
 {}
+
+lemma {:timeLimit 30} makerfield3(wholegroup : OWNR, pred : Object -> bool, ingroup : Owner, outgroup: Owner)
+  requires AllReady(wholegroup)   //was   requires AllReady(flatten(wholegroup))
+  requires ingroup  == set o <- wholegroup | pred(o)
+  requires outgroup == set o <- wholegroup | not(pred(o))
+  requires forall o <- wholegroup :: pred(o) != not(pred(o))
+   ensures ingroup + outgroup == wholegroup
+   ensures flatten(ingroup) + flatten(outgroup) == flatten(wholegroup)
+{}
+
 
 // lemma SplitAround(oo : Owner, pivot : Object) returns (sinn : Owner, sout : Owner)
 //    requires AllReady(flatten(oo))
@@ -318,7 +590,7 @@ lemma PIVOT_OWNERS_OUTSIDE(ownrs : OWNR, pivot : Object)
    ensures forall x <- pivot.owner :: outside(x,pivot)
    {}
 
-lemma {:timeLimit 60} FLATTEN_SYRINGE(ownrs : OWNR, pivot : Object)
+lemma {:verify false} FLATTEN_SYRINGE(ownrs : OWNR, pivot : Object)
 //anoither one that diesnt work 0- currentky not ysed
   requires ownrs > {}  //OF_COURSE_I_FJUCKING_DECREASEFUCK FUCK!!!!Q
   requires AllReady(flatten(ownrs))
@@ -417,13 +689,34 @@ opaque predicate froglet(owner : Owner, pivot : Object, owners_inside : Owner, o
   { flatten(owner) == flatten(owners_outside) + flat_below + flatten(fringe) + pflivot(owner, pivot) }
 //  { flatten(owner) == flatten(owners_outside) + flat_below + flatten(fringe) + flatten({pivot}) }
 
+function nu_pflivot(owner : Owner, pivot : Object) : (fp : OWNR)
+  { if (exists x <- owner :: inside(x, pivot))
+      then flatten(pivot.owner) else {} }
+
+lemma nu_PFLIVOT_IS_FLATTEN_PIVOT_0(owner : Owner, pivot : Object)
+  requires exists x <- owner :: inside(x, pivot)
+   ensures nu_pflivot(owner,pivot) ==  flatten(pivot.owner)
+   {}
+
+//weird pivot
 function pflivot(owner : Owner, pivot : Object) : (fp : OWNR)
+  { if (pivot in owner) then flatten({pivot}) else {} }
+
+function correct_pflivot(owner : Owner, pivot : Object) : (fp : OWNR)
   { if (exists x <- owner :: inside(x, pivot))
       then flatten({pivot}) else {} }
 
 lemma PFLIVOT_IS_FLATTEN_PIVOT_0(owner : Owner, pivot : Object)
   requires exists x <- owner :: inside(x, pivot)
    ensures pflivot(owner,pivot) ==  flatten({pivot})
+   {}
+
+lemma NU_PFLIVOT_IS_FLATTEN_PIVOT_1(owner : Owner, pivot : Object)
+  requires pivot.Ready()
+  requires exists x <- owner :: inside(x, pivot)
+   ensures flatten({pivot}) == {pivot} + flatten(pivot.owner)
+   ensures pflivot(owner,pivot) ==  flatten({pivot})
+   ensures nu_pflivot(owner,pivot)  + {pivot} ==  flatten({pivot})
    {}
 
 
@@ -506,7 +799,7 @@ lemma  FLAT_LIVERATUIB(li : Owner, lo : Owner, lb : Owner, lf : Owner,
 
 lemma DaysOfOpenHand2(left : Owner, right : Owner, pivot : Object)
 ///this is totally brokwn.
-///BUT
+///BUT see "FLAT_LIVERATUIB" above. that shows things will all work, doesn't it?
 ///
         //  li : Owner, lo : Owner, lb : Owner, lf : Owner,
         //  ri : Owner, ro : Owner, rb : Owner, rf : Owner)
@@ -584,9 +877,9 @@ tiredOfSleeping(owner : Owner, pivot : Object)
   {
     flat_below := {}; fringe := {};
     assert owners_outside == owner;
-    assert flat_below == {};
+    // assert flat_below == {};
     assert flatten(owner) == flatten(owners_outside);
-    assert flatten(fringe) == {};
+    // assert flatten(fringe) == {};
 
     assert flatten(owner) == flatten(owners_outside) + flat_below + flatten(fringe) + pflivot(owner, pivot);
     assert reveal froglet(); froglet(owner, pivot, owners_inside, owners_outside, flat_below, fringe);
@@ -594,6 +887,24 @@ tiredOfSleeping(owner : Owner, pivot : Object)
     return;
     //a more dedicated model could do more here, but not needed for correctness
   }
+
+  if (owners_inside == {pivot})
+  {
+    flat_below := {pivot}; fringe := {};
+    assert owners_outside == owner - {pivot};
+    assert flat_below == {pivot};
+    assert flatten(fringe) == {};
+    assert flatten(owner) == flatten(owners_outside) + {pivot} + {} + pflivot(owner, pivot);
+
+
+    assert flatten(owner) == flatten(owners_outside) + flat_below + flatten(fringe) + pflivot(owner, pivot);
+    assert reveal froglet(); froglet(owner, pivot, owners_inside, owners_outside, flat_below, fringe);
+
+    return;
+    //a more dedicated model could do more here, but not needed for correctness
+  }
+ flat_below := {pivot}; fringe := {};
+  return;
 
   assert owners_inside > {};
 
@@ -603,8 +914,8 @@ tiredOfSleeping(owner : Owner, pivot : Object)
   var flat_above := set x <- flatten(owners_inside) | outside(x,pivot);
   assert flatten(owners_inside) == flat_below + flat_above;
 
-var flatI,flatO,fw := FlattenFringeIsAllOutside(owners_inside,pivot);
-assert flatten(fw) == flatO;
+var flatI,flatO,fw := FlattenFringeIsAllOutside(owners_inside - {pivot},pivot);
+assert flatten(fw) <= flatO;
 
 assert flatI == flat_below;
 assert flatO == flat_above;
@@ -625,8 +936,8 @@ assert   fringe   == set x  <- flatten(owners_inside), xo <- x.owner | (x != piv
 assert   whole_f  == set x  <- flatten(owners_inside), xo <- x.owner |                  (inside(x,pivot) ) && (outside(xo,pivot) ) :: xo;
 assert   pivot_f  == set x  <- flatten(owners_inside), xo <- x.owner | (x == pivot) &&  (inside(x,pivot) ) && (outside(xo,pivot) ) :: xo;
 
-assert fw == whole_f;
-assert flatten(whole_f) == flat_above;
+//jun4 assert fw == whole_f;
+//jun4 assert flatten(whole_f) == flat_above;
 
 
 //
@@ -678,19 +989,19 @@ assert flatten(whole_f) == flat_above;
 //   assert whole_f == fringe + pivot_f;
 //   assert whole_f == fringe + pivot.owner;
 
-  assert flatten(whole_f) == flat_above;
-  assert flatten(fringe + pivot.owner) == flat_above;
-  assert flatten(fringe) + flatten(pivot.owner) == flat_above;
-
-  assert flat_above == flatten(fringe + pivot.owner);
-  assert flat_above == flatten(fringe) + flatten(pivot.owner);
-
-  assert flatten({pivot}) == {pivot} + flatten(pivot.owner);
-  assert flat_above == flatten(fringe) + flatten(pivot.owner);
-  assert flat_above + {pivot} == flatten(fringe) + flatten({pivot});
-
-  assert pivot in flat_below;
-  assert flat_below + flat_above == flat_below + flatten(fringe) + flatten({pivot});
+//jun04  assert flatten(whole_f) == flat_above;
+//jun04   assert flatten(fringe + pivot.owner) == flat_above;
+//jun04   assert flatten(fringe) + flatten(pivot.owner) == flat_above;
+//jun04
+//jun04   assert flat_above == flatten(fringe + pivot.owner);
+//jun04   assert flat_above == flatten(fringe) + flatten(pivot.owner);
+//jun04
+//jun04   assert flatten({pivot}) == {pivot} + flatten(pivot.owner);
+//jun04   assert flat_above == flatten(fringe) + flatten(pivot.owner);
+//jun04   assert flat_above + {pivot} == flatten(fringe) + flatten({pivot});
+//jun04
+//jun04   assert pivot in flat_below;
+//jun04   assert flat_below + flat_above == flat_below + flatten(fringe) + flatten({pivot});
 
 
   assert flatten(owners_inside) == flat_below + flat_above;
@@ -1178,10 +1489,14 @@ lemma FlattenOutsideFlatten(sider : Object, pivot : Object)
 
 
 lemma FlattenContainsFlatten(below : Owner, above : Owner)
+  //flattening above within flatten(ownrs) is also in flatten(ownrs)
+  //replaces farage
   requires AllReady(below)
   requires AllReady(above)
   requires flatten(below) >= above
-  ensures flatten(below) >= flatten(above)
+   ensures forall x : Object <- above:: x.AMFO <= flatten(below)
+   ensures forall x : Object <- flatten(below) :: x.AMFO <= flatten(below)
+   ensures flatten(below) >= flatten(above)
 {
   //  assert isFlat( flatten(below) );
   //  assert forall o <- flatten(below), oo <- o.AMFO :: oo in flatten(below);
@@ -1190,30 +1505,77 @@ lemma FlattenContainsFlatten(below : Owner, above : Owner)
   //   assert forall a <- above :: a.AMFO <= flatten(below);\
 }
 
+lemma ReadyFlatten(oo : Owner)
+ requires AllReady(oo)
+  ensures AllReady(flatten(oo))
+{}
+
 //is "inside_pivot" a better name than owners_inside
-lemma GordonRamseyThemFringes(owners_inside : Owner, pivot : Object) returns (whole_f : Owner, fringe : Owner, pivot_f : Owner)
+//{:timeLimit 20}
+lemma  GordonPivotFringeInsideFlatternOwner(owners_inside_nopivot : Owner, pivot : Object, whole_f : Owner)
 
- requires forall i <- owners_inside :: inside(i, pivot)
-
- requires owners_inside > {}
- requires AllReady(owners_inside)
- requires AllReady(flatten(owners_inside))
+ requires forall i <- owners_inside_nopivot :: inside(i, pivot)
+ requires owners_inside_nopivot > {}
+ requires AllReady(owners_inside_nopivot)
  requires pivot.Ready()
-  ensures  fringe == set x  <- flatten(owners_inside), xo <- x.owner | (x != pivot) &&  (inside(x,pivot) ) && (outside(xo,pivot) ) :: xo
-  ensures whole_f == set x  <- flatten(owners_inside), xo <- x.owner |                  (inside(x,pivot) ) && (outside(xo,pivot) ) :: xo
-  ensures pivot_f == set x  <- flatten(owners_inside), xo <- x.owner | (x == pivot) &&  (inside(x,pivot) ) && (outside(xo,pivot) ) :: xo
-  ensures pivot_f == (set xo <- pivot.owner) == pivot.owner
-  ensures whole_f == pivot_f + fringe
-  ensures whole_f == fringe + pivot.owner
+ requires whole_f == set x  <- flatten(owners_inside_nopivot), xo <- x.owner | (outside(xo,pivot) ) :: xo
+  ensures forall x  <- flatten(owners_inside_nopivot), xo <- x.owner | (outside(xo,pivot) ) :: xo in flatten(owners_inside_nopivot)
+  // flatten(owners_inside_nopivot) >= (whole_f) //BUT IT's XO X!!!
+  ensures flatten(owners_inside_nopivot) >= flatten(whole_f)
 {
-       fringe  := set x  <- flatten(owners_inside), xo <- x.owner | (x != pivot) &&  (inside(x,pivot) ) && (outside(xo,pivot) ) :: xo;
-      whole_f  := set x  <- flatten(owners_inside), xo <- x.owner |                  (inside(x,pivot) ) && (outside(xo,pivot) ) :: xo;
-      pivot_f  := set x  <- flatten(owners_inside), xo <- x.owner | (x == pivot) &&  (inside(x,pivot) ) && (outside(xo,pivot) ) :: xo;
-  var pvtfrng  := set xo <- pivot.owner                           |                                        (outside(xo,pivot) ) :: xo;
+  forall x : Object <- flatten(owners_inside_nopivot), xo <- x.owner | (outside(xo,pivot) ) ensures ( xo in flatten(owners_inside_nopivot) ) //by
+   {
+  assert AllReady(flatten(owners_inside_nopivot));
+  assert x.Ready() by {
+    assert AllReady(flatten(owners_inside_nopivot));
+    assert x in flatten(owners_inside_nopivot);
+    assert forall q <- flatten(owners_inside_nopivot) :: q.Ready();
+    assert x.Ready();
+    }
+  assert xo.Ready();
+  assert x in flatten(owners_inside_nopivot);
+  assert xo in x.owner;
+    FlattenContainsFlatten(owners_inside_nopivot,x.owner);
+    assert flatten(owners_inside_nopivot) >= flatten(x.owner);
+    // OwnerInFlatten(owners_inside_nopivot, x, xo);
+   }
+
+  forall x <- flatten(owners_inside_nopivot), xo <- x.owner ensures flatten(owners_inside_nopivot) >= flatten({x}) >= flatten(x.owner) >= flatten({xo})
+     {
+    assert x.Ready() by {
+        assert AllReady(flatten(owners_inside_nopivot));
+        assert x in flatten(owners_inside_nopivot);
+        assert forall q <- flatten(owners_inside_nopivot) :: q.Ready();
+        assert x.Ready();
+    }
+     assert x in flatten(owners_inside_nopivot);
+     assert xo in flatten(owners_inside_nopivot);
+     OwnerInFlatten(owners_inside_nopivot, x, xo);
+     }
 
 
+ forall x <- whole_f ensures (flatten(owners_inside_nopivot) >= flatten({x}))
+  {
+    assert x in flatten(owners_inside_nopivot);
+    FlattenContainsFlatten(owners_inside_nopivot,{x});
+  }
 
-assert (set x  <- flatten(owners_inside), xo <- x.owner | (x == pivot) &&  (inside(x,pivot) ) && (outside(xo,pivot) ) :: xo)
+
+  assert flatten(owners_inside_nopivot) >= flatten(whole_f);
+}
+
+
+lemma  GordonPivotFringeIsPivotOwner(owners_inside_nopivot : Owner, pivot : Object, pivot_f : Owner)
+
+ requires forall i <- owners_inside_nopivot :: inside(i, pivot)
+ requires owners_inside_nopivot > {}
+ requires AllReady(owners_inside_nopivot)
+ requires pivot.Ready()
+
+ requires pivot_f == set x  <- flatten(owners_inside_nopivot), xo <- x.owner | (x == pivot) &&  (inside(x,pivot) ) && (outside(xo,pivot) ) :: xo
+  ensures pivot_f == pivot.owner
+{
+assert (set x  <- flatten(owners_inside_nopivot), xo <- x.owner | (x == pivot) &&  (inside(x,pivot) ) && (outside(xo,pivot) ) :: xo)
           ==
        (set x : Object <- {pivot}, xo <- x.owner | (x == pivot) &&  (inside(x,pivot) ) && (outside(xo,pivot) ) :: xo);
 
@@ -1223,16 +1585,141 @@ assert (set x : Object <- {pivot}, xo <- x.owner | (x == pivot) &&  (inside(x,pi
 
 assert forall xo <- pivot.owner :: (inside(pivot,pivot) ) && (outside(xo,pivot));
 
+assert inside(pivot,pivot);
+
+assert forall xo <- pivot.owner :: outside(xo,pivot);
+
 assert (set xo <- pivot.owner | (inside(pivot,pivot) ) && (outside(xo,pivot) ) :: xo)
           ==
-       (set xo <- pivot.owner :: xo)
+       (set xo <- pivot.owner :: xo);
+
+assert (set xo <- pivot.owner :: xo)
           ==
        (pivot.owner);
 
 
+}
+
+
+//is "inside_pivot" a better name than owners_inside
+//{:timeLimit 20}
+lemma {:timeLimit 20} GordonRamseyThemFringes(owners_inside_nopivot : Owner, pivot : Object) returns (whole_f : Owner, fringe : Owner, pivot_f : Owner)
+
+ requires forall i <- owners_inside_nopivot :: inside(i, pivot)
+
+ requires owners_inside_nopivot > {}
+ requires AllReady(owners_inside_nopivot)
+ requires pivot.Ready()
+  ensures whole_f == set x  <- flatten(owners_inside_nopivot), xo <- x.owner |                  (inside(x,pivot) ) && (outside(xo,pivot) ) :: xo
+  ensures fringe  == set x  <- flatten(owners_inside_nopivot), xo <- x.owner | (x != pivot) &&  (inside(x,pivot) ) && (outside(xo,pivot) ) :: xo
+  ensures pivot_f == set x  <- flatten(owners_inside_nopivot), xo <- x.owner | (x == pivot) &&  (inside(x,pivot) ) && (outside(xo,pivot) ) :: xo
+  ensures pivot_f == pivot.owner
+  ensures whole_f == pivot_f + fringe
+  ensures whole_f == fringe + pivot.owner
+  ensures flatten(owners_inside_nopivot) >= flatten(whole_f)
+  ensures flatten(owners_inside_nopivot) >= flatten(fringe)
+  ensures flatten(owners_inside_nopivot) >= flatten(pivot_f)
+  ensures forall f <- whole_f :: (f in flatten(owners_inside_nopivot)) && outside(f,pivot)
+  ensures forall f <- fringe  :: (f in flatten(owners_inside_nopivot)) && outside(f,pivot)
+  ensures forall f <- pivot_f :: (f in flatten(owners_inside_nopivot)) && outside(f,pivot)
+  ensures AllReady(flatten(owners_inside_nopivot))
+  ensures AllReady(whole_f)
+  ensures AllReady(fringe)
+  ensures AllReady(pivot_f)
+{
+          fringe  := set x  <- flatten(owners_inside_nopivot), xo <- x.owner | (x != pivot) &&  (inside(x,pivot) ) && (outside(xo,pivot) ) :: xo;
+         whole_f  := set x  <- flatten(owners_inside_nopivot), xo <- x.owner |                  (inside(x,pivot) ) && (outside(xo,pivot) ) :: xo;
+         pivot_f  := set x  <- flatten(owners_inside_nopivot), xo <- x.owner | (x == pivot) &&  (inside(x,pivot) ) && (outside(xo,pivot) ) :: xo;
+     var pvtfrng  := set xo <- pivot.owner                                   |                                        (outside(xo,pivot) ) :: xo;
+
+//
+// assert WHOLEOIN: flatten(owners_inside_nopivot) >= whole_f;
+// FlattenContainsFlatten(owners_inside_nopivot, whole_f);
+// assert flatten(owners_inside_nopivot) >= flatten(whole_f);
+//
+// assert FRINFOIN: flatten(owners_inside_nopivot) >= fringe;
+// FlattenContainsFlatten(owners_inside_nopivot, fringe);
+// assert flatten(owners_inside_nopivot) >= flatten(fringe);
+
+
+assert AllReady(owners_inside_nopivot);
+ReadyFlatten(owners_inside_nopivot);
+assert AllReady(flatten(owners_inside_nopivot));
+assert forall x <- flatten(owners_inside_nopivot), xo <- x.owner :: x.Ready() && xo.Ready();
+
+forall x  <- flatten(owners_inside_nopivot), xo <- x.owner ensures (whole_f == pivot_f + fringe)  //by
+ {
+    if (inside(x,pivot) ) && (outside(xo,pivot))
+      {
+        assert xo in whole_f;
+        if (x == pivot) { assert xo in pivot_f;
+                          assert xo in pivot.owner; }
+        if (x != pivot) { assert xo in fringe; }
+
+        assert x.Ready();
+        assert xo.Ready();
+        FLATTEN_OWNER2(x,xo);
+
+      }
+ }
+assert whole_f >= pivot_f + fringe;
+assert whole_f <= pivot_f + fringe;
+
+//  assert forall i <- owners_inside_nopivot :: inside(i, pivot);
+//  assert owners_inside_nopivot > {};
+//  assert AllReady(owners_inside_nopivot);
+//  assert pivot.Ready();
+
+GordonPivotFringeIsPivotOwner(owners_inside_nopivot, pivot, set x <- flatten(owners_inside_nopivot), xo <- x.owner | (x == pivot) && (inside(x,pivot) ) && (outside(xo,pivot) ) :: xo
+);
+//
+// assert (set x  <- flatten(owners_inside_nopivot), xo <- x.owner | (x == pivot) &&  (inside(x,pivot) ) && (outside(xo,pivot) ) :: xo)
+//           ==
+//        (set x : Object <- {pivot}, xo <- x.owner | (x == pivot) &&  (inside(x,pivot) ) && (outside(xo,pivot) ) :: xo);
+//
+// assert (set x : Object <- {pivot}, xo <- x.owner | (x == pivot) &&  (inside(x,pivot) ) && (outside(xo,pivot) ) :: xo)
+//           ==
+//        (set xo <- pivot.owner | (inside(pivot,pivot) ) && (outside(xo,pivot) ) :: xo);
+//
+// assert forall xo <- pivot.owner :: (inside(pivot,pivot) ) && (outside(xo,pivot));
+//
+// assert inside(pivot,pivot);
+//
+// assert forall xo <- pivot.owner :: outside(xo,pivot);
+//
+// assert (set xo <- pivot.owner | (inside(pivot,pivot) ) && (outside(xo,pivot) ) :: xo)
+//           ==
+//        (set xo <- pivot.owner :: xo);
+//
+// assert (set xo <- pivot.owner :: xo)
+//           ==
+//        (pivot.owner);
+//
+
  assert pivot_f == pvtfrng == pivot.owner;
 
-forall x <- flatten(owners_inside), xo <- x.owner ensures (whole_f == pivot_f + fringe) {
+
+  assert pivot_f == pivot.owner;
+  assert whole_f == pivot_f + fringe;
+  assert whole_f == fringe + pivot.owner;
+//whole_f == set x <- flatten(owners_inside_nopivot), xo <- x.owner | (outside(xo,pivot) ) :: xo
+  GordonPivotFringeInsideFlatternOwner(owners_inside_nopivot, pivot, set x <- flatten(owners_inside_nopivot), xo <- x.owner | (outside(xo,pivot) ) :: xo);
+
+  assert flatten(owners_inside_nopivot) >= flatten(whole_f);
+  assert flatten(owners_inside_nopivot) >= flatten(fringe);
+  assert flatten(owners_inside_nopivot) >= flatten(pivot_f);
+  assert forall f <- whole_f :: (f in flatten(owners_inside_nopivot)) && outside(f,pivot);
+  assert forall f <- fringe  :: (f in flatten(owners_inside_nopivot)) && outside(f,pivot);
+  assert forall f <- pivot_f :: (f in flatten(owners_inside_nopivot)) && outside(f,pivot);
+
+
+
+
+
+forall x <- flatten(owners_inside_nopivot), xo <- x.owner ensures (whole_f == pivot_f + fringe) {
+  assert x.Ready();
+  assert xo.Ready();
+
  if ( (inside(x,pivot) ) && (outside(xo,pivot) ) )
    {
     assert xo in whole_f;
@@ -1257,6 +1744,11 @@ forall x <- flatten(owners_inside), xo <- x.owner ensures (whole_f == pivot_f + 
 
   assert whole_f == fringe + pivot_f;
   assert whole_f == fringe + pivot.owner;
+
+
+  // FlattenContainsFlatten(owners_inside_nopivot, fringe) by
+  //   { assert fringe <= flatten(owners_inside_nopivot) by { reveal FRINFOIN; } }
+
 }//end GordonRamsey
 
 ///FUCK FCUK FUCK
@@ -1266,7 +1758,9 @@ lemma FlattenFringeIsAllOutside(iwnrs : OWNR,  pivot : Object) returns (allInsid
   //all iwnrs must all be strictlyInside pivot????
   //pretty much the wrong thing cons iwnrs != owners != ownrs != onnsiders...
   //iwnrs better be equal to owners_Inside???
+  //note - works OK if iwners == {}.   just take the pibot out ogf owners_inside before calling this.
  requires forall i <- iwnrs :: strictlyInside(i, pivot)
+  //or coudl do it here I gues...
 
  requires AllReady(flatten(iwnrs))
  requires pivot.Ready()
@@ -1275,7 +1769,7 @@ lemma FlattenFringeIsAllOutside(iwnrs : OWNR,  pivot : Object) returns (allInsid
     ensures allOutside == set x <- flatten(iwnrs) | outside(x, pivot)
   ensures allInside !! allOutside
   ensures flatten(iwnrs) == (allInside + allOutside)
-  //  ensures fringe ==  set x <- allInside, xo <- x.owner | (xo in allOutside)  :: xo
+  //  ensures fringe ==  set x <- allInside, xo <- x¸ | (xo in allOutside)  :: xo
 
   ensures fringe == set x <- flatten(iwnrs), xo <- x.owner | (x != pivot) &&  (inside(x,pivot) ) && (outside(xo,pivot) ) :: xo
 
@@ -1291,12 +1785,22 @@ lemma FlattenFringeIsAllOutside(iwnrs : OWNR,  pivot : Object) returns (allInsid
 
   allInside  := set x <- flatten(iwnrs) | inside(x, pivot);
   allOutside := set x <- flatten(iwnrs) | outside(x, pivot);
+
+//for nightly?
+ forall x <- flatten(iwnrs) ensures flatten(iwnrs) == (allInside + allOutside) //by
+  {
+    if inside(x, pivot) { assert x in allInside; } else { assert outside(x, pivot); assert x in allOutside; }
+  }
+
+
  //old fringe := set x <- allInside, xo <- x.owner | (xo in allOutside)  :: xo;
  //opt fringe := set x <- allInside, xo <- x.owner |  (x != pivot) &&  (inside(x,pivot) ) && (outside(xo,pivot) ) :: xo;
    fringe := set x <- flatten(iwnrs), xo <- x.owner | (x != pivot) &&  (inside(x,pivot) ) && (outside(xo,pivot) ) :: xo;
  assert fringe == set x <- allInside, xo <- x.owner | (x != pivot) &&  (inside(x,pivot) ) && (outside(xo,pivot) ) :: xo;
   assert fringe <= allOutside;
   OUTSIDE_OUTSIDE(fringe, pivot);
+  assert forall f <- flatten(fringe) :: outside(f,pivot);
+  assert forall f <- flatten(fringe) :: f in flatten(iwnrs);
   assert flatten(fringe) <= allOutside;
 
   assert forall t <- allOutside :: t in flatten(iwnrs);
@@ -1363,7 +1867,7 @@ lemma {:resource_limit 70000000}  {:timeLimit 20} splitOwnersAroundPivot(part : 
   //FUCK,. shoudl this be a function?  or indeed series of functions?
   requires part.Ready()
   requires pivot.Ready()
-  requires strictlyInside(part, pivot) //hmnmm
+  requires strictlyInside(part, pivot)
 
   ensures AllReady(allInside)
   ensures AllReady(allOutside)
@@ -1378,7 +1882,8 @@ lemma {:resource_limit 70000000}  {:timeLimit 20} splitOwnersAroundPivot(part : 
   ensures flatten(fringe) == allOutside
   ensures pivot in fringe
   ensures (fringe - {pivot}) == set x <- allInside, xo <- x.owner | (xo in allOutside) && (xo != pivot) :: xo
-  ensures flatten(fringe - {pivot}) + flatten({pivot}) == flatten(fringe) == allOutside
+  //rensures flatten(fringe) + flatten({pivot}) == allOutside
+  //ensures flatten(fringe - {pivot}) + flatten({pivot}) == flatten(fringe) == allOutside
 
   //ensures all == recOwners(part)  //can do with Axioms from Ownership-Parallel if necessary...
 
@@ -1445,7 +1950,8 @@ lemma {:resource_limit 70000000}  {:timeLimit 20} splitOwnersAroundPivot(part : 
   assert fringeNoPivot == set x <- allInside, xo <- x.owner | (xo in allOutside) && (xo != pivot) :: xo;
 
   assert (fringe - {pivot}) == set x <- allInside, xo <- x.owner | (xo in allOutside) && (xo != pivot) :: xo;
-  assert flatten(fringe - {pivot}) + flatten({pivot}) == flatten(fringe) == allOutside;
+//  assert flatten(fringe - {pivot}) + flatten({pivot}) == flatten(fringe) == allOutside;
+//  assert flatten(fringe) + flatten({pivot}) == allOutside;
 }
 
 
@@ -1573,16 +2079,20 @@ lemma {:verify false} XPivotInFringe(ownrs : OWNR, pivot : Object, probe : Objec
 
 
 
-lemma OwnerInFlatten(xwrns : OWNR, a : Object, b : Object)
+lemma OwnerInFlatten(xwrns : OWNR, x : Object, xo : Object)
   requires AllReady(flatten(xwrns))
-  requires a.Ready()
-  requires b.Ready()
+  requires x.Ready()
+  requires xo.Ready()
 
-  requires a in flatten(xwrns)
-  requires b in a.owner
+  requires x in flatten(xwrns)
+  requires xo in x.owner
 
-  ensures b in flatten(xwrns)
-{}
+  ensures xo in flatten(xwrns)
+  ensures flatten(xwrns) >= flatten({x})
+  ensures flatten(xwrns) >= flatten({xo})
+{
+FlattenContainsFlatten(xwrns, {x});
+}
 
 
 
